*üö®üö® –í –º–∞—Ç–µ—Ä–∏–∞–ª–µ –º–æ–≥—É—Ç –±—ã—Ç—å –æ–ø–µ—á–∞—Ç–∫–∏ –∏ –æ—à–∏–±–∫–∏ üö®üö®*

*–ù–æ–≤–æ–∂–µ–Ω–æ–≤ –ü–∞–≤–µ–ª*
*–≠–ù-26*

---

–ü–æ–ª—É—á–∏–º –≤–æ–ª–Ω–æ–≤–æ–µ —É—Ä–∞–≤–Ω–µ–Ω–∏–µ –∏–∑ —Ñ—É–Ω–∫—Ü–∏–∏ –æ—Ç–∫–ª–æ–Ω–µ–Ω–∏—è –æ—Ç –ø–æ–ª–æ–∂–µ–Ω–∏—è —Ä–∞–≤–Ω–æ–≤–µ—Å–∏—è.

$$\xi(\vec r, t) = a \cos(\omega t - \vec k \vec r + \alpha)$$
$$\vec k \vec r = k_xx + k_yy + k_zz$$
$$\frac{\partial \xi}{\partial t} = - a \omega \sin(\omega t - \vec k \vec r + \alpha)$$
$$\frac{\partial^2 \xi}{\partial t^2} = - a \omega^2 \cos(\omega t - \vec k \vec r + \alpha) = -\omega^2 \xi$$

$$\frac{\partial^2 \xi}{\partial x^2} = - a k_x^2 \cos(\omega t - \vec k \vec r + \alpha) = -k_x^2\xi$$
$$\frac{\partial^2 \xi}{\partial y^2} = - a k_y^2 \cos(\omega t - \vec k \vec r + \alpha) = -k_y^2\xi$$
$$\frac{\partial^2 \xi}{\partial z^2} = - a k_z^2 \cos(\omega t - \vec k \vec r + \alpha) = -k_z^2\xi$$

$$\frac{\partial^2 \xi}{\partial x^2} + \frac{\partial^2 \xi}{\partial y^2} + \frac{\partial^2 \xi}{\partial z^2} = - (k_x^2 + k_y^2 + k_z^2) \xi$$
$$\nabla^2 \xi = - k^2 = - \frac{\omega^2}{v^2}$$
$$\nabla^2 \xi = \frac1{v^2} \frac{\partial^2 \xi}{\partial t^2} - –≤–æ–ª–Ω–æ–≤–æ–µ \ —É—Ä–∞–≤–Ω–µ–Ω–∏–µ$$

$$\xi(x, t) = f\left(t-\frac xv\right) + f\left(t+\frac xv\right)- —Ä–µ—à–µ–Ω–∏–µ \ –≤–æ–ª–Ω–æ–≤–æ–≥–æ \ —É—Ä–∞–≤–Ω–µ–Ω–∏—è$$

---

#–û–ø—Ç–∏–∫–∞